{
 "cells": [
  {
   "cell_type": "markdown",
   "id": "5eac966e-fae6-4c74-9f6b-90cd92376cd7",
   "metadata": {},
   "source": [
    "1:- Find the val%e of T(2) for the rec%rrence relation T(n) = 3T(n-1) + 12n, given that T(0)=5.\r\n",
    "105."
   ]
  },
  {
   "cell_type": "markdown",
   "id": "2e8cdea2-5ad1-4f02-b22a-c98e02dcb560",
   "metadata": {},
   "source": [
    "Given:\n",
    "T(n)=3T(n-1)+12n\n",
    "T(0)=5\n",
    "\n",
    "First Calculation T(1):\n",
    "T(1)=3t(0)+12.1\n",
    "T(1)=3.5+12\n",
    "T(1)=15+12\n",
    "T(1)=27\n",
    "\n",
    "Next, CalculateT(2):\n",
    "T(2)=3T(1)+12.2\n",
    "T(2)=3*27+24\n",
    "T(2)=105  \n",
    "\n",
    "So, the value of T(2) is 105."
   ]
  },
  {
   "cell_type": "markdown",
   "id": "1d15ae29-8f31-42d4-a349-b0a63bf2545e",
   "metadata": {},
   "source": [
    "2. Given a recrrence relation, solve it using the substitution method:\n",
    "a. T(n) = T(n-1) + c\n",
    "b. T(n) = 2T(n/2) + n\n",
    "c. T(n) = 2T(n/2) + c\n",
    "d. T(n) = T(n/2) + c"
   ]
  },
  {
   "cell_type": "markdown",
   "id": "2ec89a52-5a82-4e5f-a69f-bbb9e6f53ff4",
   "metadata": {},
   "source": [
    "a:- T(n) = T(n-1) + c\n",
    "\n",
    "Solution:-\n",
    "T(n)=T(nâˆ’1)+c\n",
    "with an initial condition \n",
    "ğ‘‡(0)=ğ‘‡(n-1)+c\n",
    "with an initial condition T(0)=T0\n",
    "Steps to Solve:\n",
    "\n",
    "1:- Substitute recursively:\n",
    "Start from ğ‘‡(ğ‘›)T(n) and express it in terms of ğ‘‡(ğ‘›âˆ’1)T(nâˆ’1):\n",
    "T(n)=T(nâˆ’1)+c\n",
    "\n",
    "2:- Substitute ğ‘‡(ğ‘›âˆ’1)T(nâˆ’1) in terms of ğ‘‡(ğ‘›âˆ’2)T(nâˆ’2):\n",
    "ğ‘‡(ğ‘›âˆ’1)=ğ‘‡(ğ‘›âˆ’2)+ğ‘\n",
    "T(nâˆ’1)=T(nâˆ’2)+c\n",
    "Therefore:\n",
    "ğ‘‡(ğ‘›)=(ğ‘‡(ğ‘›âˆ’2)+ğ‘)+ğ‘=ğ‘‡(ğ‘›âˆ’2)+2ğ‘\n",
    "T(n)=(T(nâˆ’2)+c)+c=T(nâˆ’2)+2c\n",
    "\n",
    "3:- Continue the substitution process:\n",
    "ğ‘‡(ğ‘›âˆ’2)=ğ‘‡(ğ‘›âˆ’3)+ğ‘T(nâˆ’2)=T(nâˆ’3)+c\n",
    "So:\n",
    "ğ‘‡(ğ‘›)=(ğ‘‡(ğ‘›âˆ’3)+ğ‘)+2ğ‘=ğ‘‡(ğ‘›âˆ’3)+3ğ‘\n",
    "\n",
    "4:-Generalize the pattern:\n",
    "Observing the pattern, we see:\n",
    "ğ‘‡(ğ‘›)=ğ‘‡(ğ‘›âˆ’ğ‘˜)+ğ‘˜ğ‘T(n)=T(nâˆ’k)+kc\n",
    "\n",
    "5:- Determine the value when ğ‘˜=ğ‘›:\n",
    "To express ğ‘‡(ğ‘›)T(n) in terms of the initial condition ğ‘‡0T0â€‹, set ğ‘˜=ğ‘›:\n",
    "ğ‘‡(ğ‘›)=ğ‘‡(ğ‘›âˆ’ğ‘›)+ğ‘›ğ‘\n",
    "ğ‘‡(ğ‘›)=ğ‘‡(0)+ğ‘›ğ‘\n",
    "\n",
    "6:- Substitute the initial condition:\n",
    "Given ğ‘‡(0)=ğ‘‡0T(0)=T0â€‹:\n",
    "ğ‘‡(ğ‘›)=ğ‘‡0+ğ‘›c\n",
    "\n",
    "Final Solution:\n",
    "\n",
    "The closed-form solution for the recurrence relation ğ‘‡(ğ‘›)=ğ‘‡(ğ‘›âˆ’1)+ğ‘ with the initial \n",
    "condition ğ‘‡(0)=ğ‘‡0\n",
    "is:ğ‘‡(ğ‘›)=ğ‘‡0+ğ‘›ğ‘."
   ]
  },
  {
   "cell_type": "markdown",
   "id": "e35318b0-cfdb-4bec-891c-1749e7050fbb",
   "metadata": {},
   "source": [
    "b. T(n) = 2T(n/2) + n\n",
    "Recurrence Relation:\n",
    "ğ‘‡(ğ‘›)=2ğ‘‡(ğ‘›2)+ğ‘›T(n)=2T(2nâ€‹)+n\n",
    "\n",
    "Steps to Solve:\n",
    "\n",
    "1:- Substitute recursively:\n",
    "Start by expressing T(n) in terms of ğ‘‡(ğ‘›2)T(2nâ€‹):\n",
    "T(n)=2T(2nâ€‹)+n\n",
    "\n",
    "2:- Substitute ğ‘‡(ğ‘›2)T(2nâ€‹) in terms of ğ‘‡(ğ‘›4)T(4nâ€‹):\n",
    "ğ‘‡(ğ‘›2)=2ğ‘‡(ğ‘›4)+ğ‘›2T(2nâ€‹)=2T(4nâ€‹)+2n\n",
    "â€‹Therefore:\n",
    "ğ‘‡(ğ‘›)=2(2ğ‘‡(ğ‘›4)+ğ‘›2)+ğ‘›=4T(4nâ€‹)+n+n=4T(4nâ€‹)+2n\n",
    "\n",
    "3:- Continue the substitution process:\n",
    "T(4nâ€‹)=2T(8nâ€‹)+4n\n",
    "so,\n",
    "T(n)=4(2T(8nâ€‹)+4nâ€‹)+2n=8T(8nâ€‹)+n+2n=8T(8nâ€‹)+3n\n",
    "\n",
    "4:- Generalize the pattern:\n",
    "Observing the pattern, we see:\n",
    "T(n)=2kT(2knâ€‹)+kn\n",
    "\n",
    "5:-Determine the value when ğ‘›2ğ‘˜=12knâ€‹=1:\n",
    "This happens when ğ‘›=2ğ‘˜n=2k, which means ğ‘˜=logâ¡2ğ‘›k=log2â€‹n.\n",
    "Substitute ğ‘˜=logâ¡2ğ‘›k=log2â€‹n:\n",
    "T(n)=2log2â€‹nT(2log2â€‹nnâ€‹)+(log2â€‹n)n\n",
    "T(n)=nT(1)+nlog2â€‹n\n",
    "\n",
    "6:- Substitute the base case ğ‘‡(1)T(1):\n",
    "Typically, ğ‘‡(1)T(1) is given or can be assumed as a constant ğ‘‡(1)=ğ‘T(1)=c.\n",
    "Assuming ğ‘‡(1)=ğ‘T(1)=c:\n",
    "T(n)=nc+nlog2â€‹n\n",
    "\n",
    "Final Solution:\n",
    "The closed-form solution for the recurrence relation ğ‘‡(ğ‘›)=2ğ‘‡(ğ‘›2)+ğ‘›T(n)=2T(2nâ€‹)+n with the base case:\n",
    "T(1)=c is:\n",
    "T(n)=cn+nlog2â€‹n\n",
    "This solution shows that ğ‘‡(ğ‘›)T(n) grows as ğ‘›logâ¡2ğ‘›nlog2â€‹n plus a linear term ğ‘ğ‘›cn."
   ]
  },
  {
   "cell_type": "code",
   "execution_count": null,
   "id": "f99aab71-637f-4327-b9b0-5c06a2e567e2",
   "metadata": {},
   "outputs": [],
   "source": []
  },
  {
   "cell_type": "code",
   "execution_count": null,
   "id": "3a47b966-212b-4442-8516-eede343b11d5",
   "metadata": {},
   "outputs": [],
   "source": []
  }
 ],
 "metadata": {
  "kernelspec": {
   "display_name": "Python 3 (ipykernel)",
   "language": "python",
   "name": "python3"
  },
  "language_info": {
   "codemirror_mode": {
    "name": "ipython",
    "version": 3
   },
   "file_extension": ".py",
   "mimetype": "text/x-python",
   "name": "python",
   "nbconvert_exporter": "python",
   "pygments_lexer": "ipython3",
   "version": "3.11.7"
  }
 },
 "nbformat": 4,
 "nbformat_minor": 5
}
